@prefix dc: <http://purl.org/dc/elements/1.1/> .
@prefix dcterms: <http://purl.org/dc/terms/> .
@prefix knil: <https://kurrawong.ai/vocab/nil/1.0/> .
@prefix mmon: <http://www.opengis.net/def/metamodel/ogc-na/> .
@prefix nil: <http://www.opengis.net/def/nil/OGC/0/> .
@prefix ogc: <http://www.opengis.net/def/> .
@prefix owl: <http://www.w3.org/2002/07/owl#> .
@prefix rdfs: <http://www.w3.org/2000/01/rdf-schema#> .
@prefix skos: <http://www.w3.org/2004/02/skos/core#> .
@prefix status: <http://www.opengis.net/def/status/> .
@prefix xsd: <http://www.w3.org/2001/XMLSchema#> .

knil: a skos:ConceptScheme ;
    dcterms:creator <https://orcid.org/0000-0002-3322-1868> ;
    dcterms:isVersionOf ogc:nil ;
    dcterms:modified "2025-09-02"^^xsd:date ;
    dcterms:title "Nil reasons (Kurrawong derivative v1.0)"@en ;
    rdfs:comment "Derivative work of OGC nil reasons with uppercase-only concepts and hasTopConcept relationships. Intended for contribution back to OGC."@en ;
    owl:versionInfo "1.0" .

<http://www.opengis.net/def/nil/> a skos:Collection ;
    dcterms:provenance "Generated by the OGC Definitions Server to support integration of the elements of this ConceptScheme into bigger collections. ogc_skos_profile_entailements.ttl" ;
    skos:definition "Collection hierarchy for this ConceptScheme" ;
    skos:inScheme ogc:nil ;
    skos:member <http://www.opengis.net/def/nil/OGC/>,
        <http://www.opengis.net/def/nil/ogc/>,
        <http://www.opengis.net/def/nil/ogc/0/> ;
    skos:prefLabel "Concepts in OGC nils" .

nil:AboveDetectionRange a skos:Concept ;
    dc:creator "GMLJP2 SWG" ;
    dc:date "2010-03-23"^^xsd:date ;
    dc:source "OGC 07-036 Clause 8.2.3" ;
    dcterms:created "2010-03-23"^^xsd:date ;
    dcterms:modified "2012-02-14"^^xsd:date ;
    mmon:status status:valid ;
    skos:altLabel "Above Detection Range"@en ;
    skos:definition "Value was above the detection range of the instrument used to estimate it."@en ;
    skos:inScheme ogc:nil ;
    skos:prefLabel "above detection range"@en .

nil:BelowDetectionRange a skos:Concept ;
    dc:creator "GMLJP2 SWG" ;
    dc:date "2010-03-23"^^xsd:date ;
    dc:source "OGC 07-036 Clause 8.2.3" ;
    dcterms:created "2010-03-23"^^xsd:date ;
    dcterms:modified "2012-02-14"^^xsd:date ;
    mmon:status status:valid ;
    skos:altLabel "Below Detection Range"@en ;
    skos:definition "Value was below the detection range of the instrument used to estimate it."@en ;
    skos:inScheme ogc:nil ;
    skos:prefLabel "below detection range"@en .

nil:inapplicable a skos:Concept ;
    dc:creator "GML SWG" ;
    dc:date "2010-03-23"^^xsd:date ;
    dc:source "OGC 07-036 Clause 8.2.3" ;
    dcterms:created "2010-03-23"^^xsd:date ;
    dcterms:modified "2012-02-14"^^xsd:date ;
    mmon:status status:valid ;
    skos:altLabel "Inapplicable"@en ;
    skos:definition "There is no value"@en ;
    skos:inScheme ogc:nil ;
    skos:prefLabel "inapplicable"@en .

nil:template a skos:Concept ;
    dc:creator "GML SWG" ;
    dc:date "2010-03-23"^^xsd:date ;
    dc:source "OGC 07-036 Clause 8.2.3" ;
    dcterms:created "2010-03-23"^^xsd:date ;
    dcterms:modified "2012-02-14"^^xsd:date ;
    mmon:status status:valid ;
    skos:altLabel "Template"@en ;
    skos:definition "The value will be available later"@en ;
    skos:inScheme ogc:nil ;
    skos:prefLabel "template"@en .

nil:withheld a skos:Concept ;
    dc:creator "GML SWG" ;
    dc:date "2010-03-23"^^xsd:date ;
    dc:source "OGC 07-036 Clause 8.2.3" ;
    dcterms:created "2010-03-23"^^xsd:date ;
    dcterms:modified "2012-02-14"^^xsd:date ;
    mmon:status status:valid ;
    skos:altLabel "Withheld"@en ;
    skos:definition "The value is not divulged."@en ;
    skos:inScheme ogc:nil ;
    skos:prefLabel "withheld"@en .

nil:missing a skos:Concept ;
    dc:creator "GML SWG" ;
    dc:date "2010-03-23"^^xsd:date ;
    dc:source "OGC 07-036 Clause 8.2.3" ;
    dcterms:created "2010-03-23"^^xsd:date ;
    dcterms:modified "2012-02-14"^^xsd:date ;
    mmon:status status:valid ;
    rdfs:comment "More details are available via the exactMatch reference, which should be used for citation by preference"@en ;
    skos:altLabel "Missing"@en ;
    skos:definition "The correct value is not readily available to the sender of this data. Furthermore, a correct value may not exist"@en ;
    skos:exactMatch <http://www.opengis.net/def/waterml/2.0/quality/missing> ;
    skos:inScheme ogc:nil,
        ogc:waterml ;
    skos:prefLabel "missing"@en .

nil:unknown a skos:Concept ;
    dc:creator "GML SWG" ;
    dc:date "2010-03-23"^^xsd:date ;
    dc:source "OGC 07-036 Clause 8.2.3" ;
    dcterms:created "2010-03-23"^^xsd:date ;
    dcterms:modified "2012-02-14"^^xsd:date ;
    mmon:status status:valid ;
    rdfs:comment "More details are available via the exactMatch reference, which should be used for citation by preference"@en ;
    skos:altLabel "Unknown"@en ;
    skos:definition "The correct value is not known to, or not computable by, the sender of this data. However, the correct value probably exists"@en ;
    skos:exactMatch <http://www.opengis.net/def/waterml/2.0/medium/Unknown> ;
    skos:inScheme ogc:nil,
        ogc:waterml ;
    skos:prefLabel "unknown"@en .

ogc:waterml skos:hasTopConcept nil:missing,
        nil:unknown .

ogc:nil a owl:Ontology,
        skos:ConceptScheme ;
    dc:creator "Rob Atkinson, OGC" ;
    dc:rights "Copyright Â© 2012 Open Geospatial Consortium, Inc. All Rights Reserved." ;
    dc:source "8.2.3.1 in OGC 07-036 (GML)" ;
    dc:title "Nil reasons" ;
    dcterms:created "2012-02-15"^^xsd:date ;
    dcterms:modified "2023-03-23"^^xsd:date ;
    dcterms:rights <http://www.opengeospatial.org/ogc/software> ;
    dcterms:source <http://www.opengis.net/def/entities/bodies/ogcna> ;
    mmon:collectionView <http://www.opengis.net/def/nil/>,
        <http://www.opengis.net/def/ogc/> ;
    rdfs:comment "The URIs for resources in this document were assigned in accordance with the OGC Naming policies, overseen by the OGC Naming Authority. They are not otherwise managed as part of a delegated governance via a specific artefact, such as CodeLists from a normative schema." ;
    owl:imports ogc:ogc-na ;
    skos:definition "OGC nils" ;
    skos:hasTopConcept nil:AboveDetectionRange,
        nil:BelowDetectionRange,
        nil:inapplicable,
        nil:missing,
        nil:template,
        nil:unknown,
        nil:withheld ;
    skos:historyNote "refactored from original omnibus concept scheme into a separate scheme for reuse" ;
    skos:prefLabel "OGC nils" .

